add valueflag to ElimFunc

src/ElimFunc.v
@@ -5,7 +5,7 @@ Require Import Monads.
 Require Import ListLemmas.
 Require Import Psatz.
 Require Import StepLib.
-Require HigherValue.
+Require Import HigherValue.
 
 Definition function_name := nat.
 
@@ -15,85 +15,33 @@ Definition function_name := nat.
 Definition rec_info := list bool.
 
 Inductive expr :=
+| Value (v : value)
 | Arg : expr
 | UpVar : nat -> expr
 | Call : expr -> expr -> expr
-| Constr (tag : nat) (args : list expr)
+| MkConstr (tag : nat) (args : list expr)
 | ElimBody (rec : expr) (cases : list (expr * rec_info))
-| Close (f : function_name) (free : list expr)
-| CloseDyn (f : function_name) (drop : nat) (expect : nat)
+| MkClose (f : function_name) (free : list expr)
+| MkCloseDyn (f : function_name) (drop : nat) (expect : nat)
 .
 
 Definition env := list expr.
 
-Inductive value : expr -> Prop :=
-| VConstr : forall tag args, Forall value args -> value (Constr tag args)
-| VClose : forall f free, Forall value free -> value (Close f free).
+Inductive is_value : expr -> Prop :=
+| IsValue : forall v, is_value (Value v).
 
 
 Fixpoint unroll_elim (rec : expr)
                      (case : expr)
-                     (args : list expr)
+                     (args : list value)
                      (info : rec_info) : option expr :=
     match args, info with
     | [], [] => Some case
     | arg :: args, r :: info =>
-            let case := Call case arg in
-            let case := if r then Call case (Call rec arg) else case in
+            let case := Call case (Value arg) in
+            let case := if r then Call case (Call rec (Value arg)) else case in
             unroll_elim rec case args info
     | _, _ => None
-    end.
-
-
-(* Demo *)
-
-Definition add_lam_a :=             0.
-Definition add_lam_b :=             1.
-Definition elim_zero_lam_b :=       2.
-Definition elim_succ_lam_a :=       3.
-Definition elim_succ_lam_IHa :=     4.
-Definition elim_succ_lam_b :=       5.
-Definition nat_elim :=              6.
-
-Definition add_reflect := Close add_lam_a [].
-
-Definition add_env : list expr :=
-    (* add_lam_a *)
-    [ Close add_lam_b [Arg]
-    (* add_lam_b *)
-    ; Call (Call (Close nat_elim [Arg; UpVar 0]) (UpVar 0)) Arg
-    (* elim_zero_lam_b *)
-    ; Arg
-    (* elim_succ_lam_a *)
-    ; Close elim_succ_lam_IHa [Arg; UpVar 0; UpVar 1]
-    (* elim_succ_lam_IHa *)
-    ; Close elim_succ_lam_b [Arg; UpVar 0; UpVar 1; UpVar 2]
-    (* elim_succ_lam_b *)
-    ; Call (UpVar 0) (Constr 1 [Arg])
-    (* nat_elim *)
-    ; ElimBody
-        (Close nat_elim [UpVar 0; UpVar 1])
-        [(Close elim_zero_lam_b [UpVar 0; UpVar 1], []);
-         (Close elim_succ_lam_a [UpVar 0; UpVar 1], [true])]
-    ].
-
-(* Note on compilation of Elim:
-   - The Elim cases must be shifted: Arg -> UpVar0, UpVar0 -> UpVar1, etc.
-     Then the call to the newly generated function must have upvars set to
-     [Arg; UpVar0; UpVar1; ...] up to the number of used upvars.
-   - The `rec` argument should refer to the newly generated function, with
-     upvars set to [UpVar0; UpVar1; ...] up to the number of used upvars.
-   - The target is always (implicitly) Arg.  Also, upon entering a case, Arg is
-     *removed* from the local context, and everything is shifted down.  Later
-     we will no-op "compile" to another semantics that doesn't do that.
- *)
-
-Definition add_prog := (add_reflect, add_env).
-
-Fixpoint nat_reflect n : expr :=
-    match n with
-    | 0 => Constr 0 []
-    | S n => Constr 1 [nat_reflect n]
     end.
 
 
@@ -107,13 +55,14 @@ Definition expr_rect_mut
         (Pl : list expr -> Type)
         (Pp : expr * rec_info -> Type)
         (Plp : list (expr * rec_info) -> Type)
+    (HValue :   forall v, P (Value v))
     (HArg :     P Arg)
     (HUpVar :   forall n, P (UpVar n))
     (HCall :    forall f a, P f -> P a -> P (Call f a))
-    (HConstr :  forall tag args, Pl args -> P (Constr tag args))
+    (HConstr :  forall tag args, Pl args -> P (MkConstr tag args))
     (HElimBody : forall rec cases, P rec -> Plp cases -> P (ElimBody rec cases))
-    (HClose :   forall f free, Pl free -> P (Close f free))
-    (HCloseDyn : forall f drop expect, P (CloseDyn f drop expect))
+    (HClose :   forall f free, Pl free -> P (MkClose f free))
+    (HCloseDyn : forall f drop expect, P (MkCloseDyn f drop expect))
     (Hnil :     Pl [])
     (Hcons :    forall e es, P e -> Pl es -> Pl (e :: es))
     (Hpair :    forall e r, P e -> Pp (e, r))
@@ -135,13 +84,14 @@ Definition expr_rect_mut
             | p :: ps => Hcons_p p ps (go_pair p) (go_pair_list ps)
             end in
         match e as e_ return P e_ with
+        | Value v => HValue v
         | Arg => HArg
         | UpVar n => HUpVar n
         | Call f a => HCall f a (go f) (go a)
-        | Constr tag args => HConstr tag args (go_list args)
+        | MkConstr tag args => HConstr tag args (go_list args)
         | ElimBody rec cases => HElimBody rec cases (go rec) (go_pair_list cases)
-        | Close f free => HClose f free (go_list free)
-        | CloseDyn f drop expect => HCloseDyn f drop expect
+        | MkClose f free => HClose f free (go_list free)
+        | MkCloseDyn f drop expect => HCloseDyn f drop expect
         end in go e.
 
 Definition expr_rect_mut'
@@ -149,13 +99,14 @@ Definition expr_rect_mut'
         (Pl : list expr -> Type)
         (Pp : expr * rec_info -> Type)
         (Plp : list (expr * rec_info) -> Type)
+    (HValue :   forall v, P (Value v))
     (HArg :     P Arg)
     (HUpVar :   forall n, P (UpVar n))
     (HCall :    forall f a, P f -> P a -> P (Call f a))
-    (HConstr :  forall tag args, Pl args -> P (Constr tag args))
+    (HConstr :  forall tag args, Pl args -> P (MkConstr tag args))
     (HElimBody : forall rec cases, P rec -> Plp cases -> P (ElimBody rec cases))
-    (HClose :   forall f free, Pl free -> P (Close f free))
-    (HCloseDyn : forall f drop expect, P (CloseDyn f drop expect))
+    (HClose :   forall f free, Pl free -> P (MkClose f free))
+    (HCloseDyn : forall f drop expect, P (MkCloseDyn f drop expect))
     (Hnil :     Pl [])
     (Hcons :    forall e es, P e -> Pl es -> Pl (e :: es))
     (Hpair :    forall e r, P e -> Pp (e, r))
@@ -166,7 +117,7 @@ Definition expr_rect_mut'
     (forall p, Pp p) *
     (forall ps, Plp ps) :=
     let go := expr_rect_mut P Pl Pp Plp
-        HArg HUpVar HCall HConstr HElimBody HClose HCloseDyn
+        HValue HArg HUpVar HCall HConstr HElimBody HClose HCloseDyn
         Hnil Hcons Hpair Hnil_p Hcons_p in
     let fix go_list es :=
         match es as es_ return Pl es_ with
@@ -185,34 +136,36 @@ Definition expr_rect_mut'
 
 (* Useful wrapper for `expr_rect_mut with (Pl := Forall P)` *)
 Definition expr_ind' (P : expr -> Prop) (Pp : (expr * rec_info) -> Prop)
+    (HValue :   forall v, P (Value v))
     (HArg :     P Arg)
     (HUpVar :   forall n, P (UpVar n))
     (HCall :    forall f a, P f -> P a -> P (Call f a))
-    (HConstr :  forall c args, Forall P args -> P (Constr c args))
+    (HConstr :  forall c args, Forall P args -> P (MkConstr c args))
     (HElimBody : forall rec cases,
         P rec -> Forall Pp cases -> P (ElimBody rec cases))
-    (HClose :   forall f free, Forall P free -> P (Close f free))
-    (HCloseDyn : forall f drop expect, P (CloseDyn f drop expect))
+    (HClose :   forall f free, Forall P free -> P (MkClose f free))
+    (HCloseDyn : forall f drop expect, P (MkCloseDyn f drop expect))
     (Hpair :    forall e r, P e -> Pp (e, r))
     (e : expr) : P e :=
     ltac:(refine (@expr_rect_mut P (Forall P) Pp (Forall Pp)
-        HArg HUpVar HCall HConstr HElimBody HClose HCloseDyn _ _ Hpair _ _ e); eauto).
+        HValue HArg HUpVar HCall HConstr HElimBody HClose HCloseDyn _ _ Hpair _ _ e); eauto).
 
 (* Useful wrapper for `expr_rect_mut with (Pl := Forall P)` *)
 Definition expr_ind'' (P : expr -> Prop)
+    (HValue :   forall v, P (Value v))
     (HArg :     P Arg)
     (HUpVar :   forall n, P (UpVar n))
     (HCall :    forall f a, P f -> P a -> P (Call f a))
-    (HConstr :  forall c args, Forall P args -> P (Constr c args))
+    (HConstr :  forall c args, Forall P args -> P (MkConstr c args))
     (HElimBody : forall rec cases,
         P rec ->
         Forall (fun c => P (fst c)) cases ->
         P (ElimBody rec cases))
-    (HClose :   forall f free, Forall P free -> P (Close f free))
-    (HCloseDyn : forall f drop expect, P (CloseDyn f drop expect))
+    (HClose :   forall f free, Forall P free -> P (MkClose f free))
+    (HCloseDyn : forall f drop expect, P (MkCloseDyn f drop expect))
     (e : expr) : P e :=
     ltac:(refine (@expr_rect_mut P (Forall P) (fun c => P (fst c)) (Forall (fun c => P (fst c)))
-        HArg HUpVar HCall HConstr HElimBody HClose HCloseDyn _ _ _ _ _ e); eauto).
+        HValue HArg HUpVar HCall HConstr HElimBody HClose HCloseDyn _ _ _ _ _ e); eauto).
 
 
 (*
@@ -236,14 +189,15 @@ Definition num_locals :=
             | p :: ps => max (go_pair p) (go_list_pair ps)
             end in
         match e with
+        | Value _ => 0
         | Arg => 1
         | UpVar i => S (S i)
         | Call f a => max (go f) (go a)
-        | Constr _ args => go_list args
+        | MkConstr _ args => go_list args
         (* Recall: ElimBody implicitly accesses Arg, and removes it before running cases *)
         | ElimBody rec cases => max (max (go rec) (S (go_list_pair cases))) 1
-        | Close _ free => go_list free
-        | CloseDyn _ drop expect => if eq_nat_dec expect 0 then 0 else drop + expect
+        | MkClose _ free => go_list free
+        | MkCloseDyn _ drop expect => if eq_nat_dec expect 0 then 0 else drop + expect
         end in go.
 
 (* Nested fixpoint aliases *)
@@ -285,18 +239,8 @@ Lemma num_locals_list_pair_is_maximum : forall es,
 induction es; simpl in *; try destruct a; eauto.
 Qed.
 
-Lemma value_num_locals : forall e, value e -> num_locals e = 0.
-induction e using expr_ind''; intros0 Hval; invc Hval;
-simpl; refold_num_locals;
-rewrite num_locals_list_is_maximum.
-
-- cut (maximum (map num_locals args) <= 0). { intro. lia. }
-  rewrite maximum_le_Forall, <- Forall_map. list_magic_on (args, tt).
-  firstorder lia.
-
-- cut (maximum (map num_locals free) <= 0). { intro. lia. }
-  rewrite maximum_le_Forall, <- Forall_map. list_magic_on (free, tt).
-  firstorder lia.
+Lemma value_num_locals : forall e, is_value e -> num_locals e = 0.
+inversion 1. reflexivity.
 Qed.
 
 
@@ -304,8 +248,8 @@ Qed.
 (* Continuation-based step relation *)
 
 Inductive state :=
-| Run (e : expr) (l : list expr) (k : expr -> state)
-| Stop (e : expr).
+| Run (e : expr) (l : list value) (k : value -> state)
+| Stop (e : value).
 
 Inductive sstep (E : env) : state -> state -> Prop :=
 | SArg : forall l k v,
@@ -316,50 +260,47 @@ Inductive sstep (E : env) : state -> state -> Prop :=
         sstep E (Run (UpVar n) l k) (k v)
 
 | SCloseStep : forall fname vs e es l k,
-        Forall value vs ->
-        ~ value e ->
-        sstep E (Run (Close fname (vs ++ [e] ++ es)) l k)
-                (Run e l (fun v => Run (Close fname (vs ++ [v] ++ es)) l k))
+        Forall is_value vs ->
+        ~ is_value e ->
+        sstep E (Run (MkClose fname (vs ++ [e] ++ es)) l k)
+                (Run e l (fun v => Run (MkClose fname (vs ++ [Value v] ++ es)) l k))
 | SCloseDone : forall fname vs l k,
-        Forall value vs ->
-        sstep E (Run (Close fname vs) l k) (k (Close fname vs))
+        let es := map Value vs in
+        sstep E (Run (MkClose fname es) l k) (k (Close fname vs))
 
 | SCloseDyn : forall fname drop expect l k,
-        sstep E (Run (CloseDyn fname drop expect) l k)
+        sstep E (Run (MkCloseDyn fname drop expect) l k)
                 (k (Close fname (skipn drop l)))
 
 | SConstrStep : forall fname vs e es l k,
-        Forall value vs ->
-        ~ value e ->
-        sstep E (Run (Constr fname (vs ++ [e] ++ es)) l k)
-                (Run e l (fun v => Run (Constr fname (vs ++ [v] ++ es)) l k))
+        Forall is_value vs ->
+        ~ is_value e ->
+        sstep E (Run (MkConstr fname (vs ++ [e] ++ es)) l k)
+                (Run e l (fun v => Run (MkConstr fname (vs ++ [Value v] ++ es)) l k))
 | SConstrDone : forall fname vs l k,
-        Forall value vs ->
-        sstep E (Run (Constr fname vs) l k) (k (Constr fname vs))
+        let es := map Value vs in
+        sstep E (Run (MkConstr fname es) l k) (k (Constr fname vs))
 
 | SCallL : forall e1 e2 l k,
-        ~ value e1 ->
+        ~ is_value e1 ->
         sstep E (Run (Call e1 e2) l k)
-                (Run e1 l (fun v => Run (Call v e2) l k))
+                (Run e1 l (fun v => Run (Call (Value v) e2) l k))
 | SCallR : forall e1 e2 l k,
-        value e1 ->
-        ~ value e2 ->
+        is_value e1 ->
+        ~ is_value e2 ->
         sstep E (Run (Call e1 e2) l k)
-                (Run e2 l (fun v => Run (Call e1 v) l k))
+                (Run e2 l (fun v => Run (Call e1 (Value v)) l k))
 | SMakeCall : forall fname free arg l k body,
-        Forall value free ->
-        value arg ->
         nth_error E fname = Some body ->
-        sstep E (Run (Call (Close fname free) arg) l k)
+        sstep E (Run (Call (Value (Close fname free)) (Value arg)) l k)
                 (Run body (arg :: free) k)
 
 | SElimStepRec : forall rec cases l k,
-        ~ value rec ->
+        ~ is_value rec ->
         sstep E (Run (ElimBody rec cases) l k)
-                (Run rec l (fun v => Run (ElimBody v cases) l k))
+                (Run rec l (fun v => Run (ElimBody (Value v) cases) l k))
 | SEliminate : forall rec cases tag args l k case info e',
-        value rec ->
-        Forall value args ->
+        is_value rec ->
         nth_error cases tag = Some (case, info) ->
         unroll_elim rec case args info = Some e' ->
         (* XXX this step *removes* the scrutinee from the local context!
@@ -387,33 +328,19 @@ Require Import Metadata.
 Definition prog_type : Type := list expr * list metadata.
 Definition valtype := HigherValue.value.
 
-Inductive expr_value : expr -> valtype -> Prop :=
-| EvConstr : forall tag args1 args2,
-        Forall2 expr_value args1 args2 ->
-        expr_value (Constr tag args1)
-                   (HigherValue.Constr tag args2)
-| EvClose : forall tag free1 free2,
-        Forall2 expr_value free1 free2 ->
-        expr_value (Close tag free1)
-                   (HigherValue.Close tag free2)
-.
-
 Inductive is_callstate (prog : prog_type) : valtype -> valtype -> state -> Prop :=
-| IsCallstate : forall fname free free_e av ae body,
+| IsCallstate : forall fname free av body,
         nth_error (fst prog) fname = Some body ->
         let fv := HigherValue.Close fname free in
-        expr_value ae av ->
-        Forall2 expr_value free_e free ->
         HigherValue.public_value (snd prog) fv ->
         HigherValue.public_value (snd prog) av ->
         is_callstate prog fv av
-            (Run body (ae :: free_e) Stop).
+            (Run body (av :: free) Stop).
 
 Inductive final_state (prog : prog_type) : state -> valtype -> Prop :=
-| FinalState : forall e v,
-        expr_value e v ->
+| FinalState : forall v,
         HigherValue.public_value (snd prog) v ->
-        final_state prog (Stop e) v.
+        final_state prog (Stop v) v.
 
 Definition initial_env (prog : prog_type) : env := fst prog.
 
@@ -442,15 +369,16 @@ Definition close_dyn_placement :=
             | p :: ps => go_pair p /\ go_list_pair ps
             end in
         match e with
+        | Value _ => True
         | Arg => True
         | UpVar _ => True
-        | Call (CloseDyn _ _ _) a => go a
+        | Call (MkCloseDyn _ _ _) a => go a
         | Call f a => go f /\ go a
-        | Constr _ args => go_list args
-        | ElimBody (CloseDyn _ _ _) cases => go_list_pair cases
+        | MkConstr _ args => go_list args
+        | ElimBody (MkCloseDyn _ _ _) cases => go_list_pair cases
         | ElimBody rec cases => go rec /\ go_list_pair cases
-        | Close _ free => go_list free
-        | CloseDyn _ _ _ => False
+        | MkClose _ free => go_list free
+        | MkCloseDyn _ _ _ => False
         end in go.
 
 Definition close_dyn_placement_list :=
@@ -491,8 +419,10 @@ induction e using expr_rect_mut with
 
 - left. constructor.
 
+- left. constructor.
+
 - destruct e1.
-  Focus 7. {
+  Focus 8. {
     destruct IHe2; [ | right; intro; auto ].
     left. auto.
   } Unfocus.
@@ -503,7 +433,7 @@ induction e using expr_rect_mut with
 - simpl. refold_close_dyn_placement. auto.
 
 - destruct e.
-  Focus 7. {
+  Focus 8. {
     simpl. refold_close_dyn_placement. auto.
   } Unfocus.
   all: destruct IHe; [ | right; inversion 1; auto ].
@@ -533,58 +463,3 @@ induction e using expr_rect_mut with
 
 Defined.
 
-
-
-
-Lemma expr_value_value : forall e v,
-    expr_value e v ->
-    value e.
-mut_induction e using expr_rect_mut' with
-    (Pl := fun es => forall vs,
-        Forall2 expr_value es vs ->
-        Forall value es)
-    (Pp := fun e : _ * rec_info => forall v,
-        expr_value (fst e) v ->
-        value (fst e))
-    (Plp := fun (es : list (_ * rec_info)) => forall vs,
-        Forall2 (fun e v => expr_value (fst e) v) es vs ->
-        Forall (fun e => value (fst e)) es);
-[intros0 Hev; try solve [invc Hev + simpl in *; eauto].. | ].
-
-- invc Hev. constructor. eauto.
-- invc Hev. constructor. eauto.
-
-- finish_mut_induction expr_value_value using list pair list_pair.
-Qed exporting.
-Hint Resolve expr_value_value.
-Hint Resolve expr_value_value_list.
-
-Lemma expr_value_inj : forall e v1 v2,
-    expr_value e v1 ->
-    expr_value e v2 ->
-    v1 = v2.
-mut_induction e using expr_rect_mut' with
-    (Pl := fun es => forall vs1 vs2,
-        Forall2 expr_value es vs1 ->
-        Forall2 expr_value es vs2 ->
-        vs1 = vs2)
-    (Pp := fun (p : expr * rec_info) => True)
-    (Plp := fun (ps : list (expr * rec_info)) => True);
-[ eauto; intros0 Hv1 Hv2; invc Hv1; invc Hv2; f_equal; eauto.. | ].
-
-- finish_mut_induction expr_value_inj using list pair list_pair.
-Qed exporting.
-
-Lemma expr_value_sur : forall v e1 e2,
-    expr_value e1 v ->
-    expr_value e2 v ->
-    e1 = e2.
-mut_induction v using HigherValue.value_rect_mut' with
-    (Pl := fun vs => forall es1 es2,
-        Forall2 expr_value es1 vs ->
-        Forall2 expr_value es2 vs ->
-        es1 = es2);
-[ eauto; intros0 Hv1 Hv2; invc Hv1; invc Hv2; f_equal; eauto.. | ].
-
-- finish_mut_induction expr_value_sur using list.
-Qed exporting.
